mppa/Machregs.v
@@ -3,7 +3,7 @@
 (*              The Compcert verified compiler                         *)
 (*                                                                     *)
 (*          Xavier Leroy, INRIA Paris-Rocquencourt                     *)
-(*          Gergö Barany, INRIA Paris-Rocquencourt                     *)
+(*          Gergö Barany, INRIA Paris                                  *)
 (*                                                                     *)
 (*  Copyright Institut National de Recherche en Informatique et en     *)
 (*  Automatique.  All rights reserved.  This file is distributed       *)
